<div class="topSpace"></div>

Date Created: 10/04/25
References: #Ref/AlgTop 
Tags: #Type/Definition

Proved by: <i>Not Applicable</i>
References: <i>Not Applicable</i>
Justifications: <i>Not Applicable</i>

Specializations: <i>Not Applicable</i>
Generalizations: <i>Not Applicable</i>
Examples: <i>Not Applicable</i>

# Simplex

``` ad-Definition
title: Definition (Simplex).

Let $v_0, \dots, v_n \in \R^{n+1}$ with [[convex hull]] $$\Konv (v_0, \dots, v_n) = \left\{ \sum_{i=1}^n t_i v_i \mid \sum_{i=0}^n t_i=1, t_i \geq 0 \right\}.$$ We call this the <ins>simplex</ins> generated by $v_0, \dots, v_n$ if the vectors $v_1-v_0, \dots, v_n -v_0$ are [[linearly independent|linearly independent]] and denote it by $\simp (v_0, \dots, v_n)$.

```

We denote the standard topological $n$-simplex by $\Delta^n := \simp (e_0, \dots, e_n)$ where the $e_i \in \R^{n+1}$ are given by $\{e_i\}_j := \delta_{i, j-1}$. $\Delta^0$ is just a point $e_0$, $\Delta^1$ is a line segment between $e_0$ and $e_1$, $\Delta^2$ is a triangle in $\R^3$ and $\Delta^4$ is [[isomorphism|isomorphic]] to a [[tetrahedron]]. 

```tikz
\usepackage{tikz}
\begin{document}
\begin{tikzpicture}[scale=3]
	\draw[->] (0,0) -- (1.5,0);
	\draw[->] (0,0) -- (0,1.5);
	\draw[red, very thick] (0,1) -- (1,0);
	\draw (0.6, 0.6) node[red] {$\Delta^2$};
	\end{tikzpicture}
\end{document}
```

A coordinate description is given by $$\Delta^n = \left\{ (t_0, \dots, t_n) \sub \R^{n+1} \mid \sum t_i = 1, t_i \geq 0 \right\}.$$ The boundary $\partial \Delta$ of an $n$-simplex is given by $n+1$ copies of $\Delta^{n-1}$.

# Face Maps

The simplex $\Delta^n$ comes with <ins>face maps</ins> $$d_i = d_i^{n-1}: \Delta^{n-1} \hookrightarrow \Delta^n$$ $$(t_0, \dots, t_{n-1}) \mapsto (t_0, \dots, t_{i-1},0,t_i, \dots, t_{n-1}).$$ The image of $d_i^{n-1}$ in $\Delta^n$ is the face opposite to $e_i$. It is a simplex generated by $e_0, \dots, e_{i-1}, e_{i+1}, \dots, e_n$.

``` ad-Proposition
title: Proposition (Chained Face Maps).

For face maps, the following rule holds for all $0 \leq j < i \leq n$: $$d_i^{n-1} d_j^{n-2} = d_j^{n-1}d_{i-1}^{n-2}.$$

```
*Proof.*
Both expressions yield $$d_i^{n-1}d_j^{n-2}(t_0, \dots, t_{n-2}) = (t_0, \dots, t_{j-1},0,\dots, t_{i-2},0,\dots,t_{n-2})=d_j^{n-1}d_{i-1}^{n-2}(t_0,\dots, t_{n-2}).$$<span style="float:right;">$\blacksquare$</span>